Changes to dynamic semantics and substitution preserves typing Lemmas

src/Language/PlutusIR/Semantics/Dynamic/Bigstep/EvalValue.v
@@ -1,47 +1,31 @@
 Require Import PlutusCert.Language.PlutusIR.
 Import NamedTerm.
+
 Require Import PlutusCert.Language.PlutusIR.Semantics.Dynamic.Bigstep.
 
-Definition P_value (v : Term) := v =[0]=> v.
-Definition P_value_builtin (v : Term) := v =[0]=> v.
-#[export] Hint Unfold P_value P_value_builtin : core.
+Require Import Lia.
 
-Lemma eval_value : forall v,
-    value v -> 
-    P_value v.
-Proof.
-  induction 1; intros; autounfold.
-  - (* V_TyAbs *) 
-    apply E_TyAbs.
-  - (* V_LamAbs *)
-    apply E_LamAbs.
-  - (* V_Constant *)
-    apply E_Constant.
-  - (* V_Error *)
-    apply E_Error.
-  - (* V_IWrap *)
-    apply E_IWrap.
-    assumption.
-  - (* V_If *)
-    apply E_If.
-  - (* V_IfTyInst *)
-    apply E_IfTyInst.
-    apply E_If.
-  - (* V_IfCondition *)
-    replace 0 with (0 + 0) by reflexivity.
-    apply E_IfCondition.
-    + apply E_IfTyInst.
-      apply E_If.
-    + apply E_Constant.
-  - (* V_IfThenBranch *)
-    apply E_IfThenBranch.
-    replace 0 with (0 + 0) by reflexivity.
-    apply E_IfCondition.
-    * apply E_IfTyInst.
-      apply E_If.
-    * apply E_Constant.
-  - (* ExtBuiltin *)
-    intros. unfold P_value_builtin.
-    apply E_ExtBuiltinPartiallyApplied.
-    assumption.
+Definition P_value (v : Term) := v =[0]=> v.
+Definition P_neutral_value (n : nat) (nv : Term) := nv =[0]=> nv.
+#[export] Hint Unfold P_value P_neutral_value : core.
+
+Lemma eval_value : 
+  (forall v, value v -> P_value v) /\
+  (forall n v, neutral_value n v -> P_neutral_value n v).
+Proof with (autounfold; (eauto || (try lia))).
+  apply value__multind.
+  all: intros.
+  all: autounfold.
+  all: try solve [constructor; eauto].
+  - inversion H; subst...
+  - inversion H2; subst.
+    all: econstructor...
+    all: econstructor...
+    all: econstructor...
+    all: eapply neutral_value__monotone...
+  - inversion H; subst.
+    all: econstructor...
+    all: econstructor...
+    all: econstructor...
+    all: eapply neutral_value__monotone...
 Qed.
