src/Language/PlutusIR/Semantics/TypeSafety/SubstitutionPreservesTyping/AnnotationSubstitution.v
@@ -1,238 +1,101 @@
 Require Import PlutusCert.Language.PlutusIR.Semantics.Static.
 Require Import PlutusCert.Language.PlutusIR.Semantics.Dynamic.
-Require Import PlutusCert.Language.PlutusIR.Semantics.TypeSafety.NormalisationPreservesKinding.
 Require Import PlutusCert.Language.PlutusIR.Semantics.TypeSafety.SubstitutionPreservesTyping.TypeSubstitution.
+
+Require Import PlutusCert.Util.Map.Mupdate.
 
 Require Import Coq.Logic.FunctionalExtensionality.
 
-Definition upd (a : tyname) (T' : Ty ) (Gamma : partial_map Ty) :=
+Definition gsubst (a : tyname) (T' : Ty ) (Gamma : partial_map Ty) :=
   fun x =>
     match Gamma x with
     | None => None
     | Datatypes.Some T => Datatypes.Some (substituteT a T' T)
     end.
 
-Lemma upd_empty : forall X U,
-    upd X U empty = empty.
+Lemma gsubst_empty : forall X U,
+    gsubst X U empty = empty.
 Proof.
   intros X U.
-  unfold upd.
+  unfold gsubst.
   simpl.
   reflexivity.
 Qed.
 
-Lemma upd__substituteT : forall Gamma x X U T,
+Lemma gsubst__substituteT : forall Gamma x X U T,
     Gamma x = Datatypes.Some T ->
-    (upd X U Gamma) x = Datatypes.Some (substituteT X U T).
+    (gsubst X U Gamma) x = Datatypes.Some (substituteT X U T).
 Proof.
   intros.
-  unfold upd.
+  unfold gsubst.
   rewrite H.
   reflexivity.
 Qed.
 
-Lemma upd_absorbs_substituteT : forall x X U T Gamma,
-    (x |-> (substituteT X U T); upd X U Gamma) = upd X U (x |-> T; Gamma).
+Lemma gsubst_absorbs_substituteT : forall x X U T Gamma,
+    (x |-> (substituteT X U T); gsubst X U Gamma) = gsubst X U (x |-> T; Gamma).
 Proof.
   intros.
   simpl.
   f_equal.
   apply functional_extensionality.
   intros.
-  destruct (x =? x0) eqn:Heqb.
+  destruct (x =? x0)%string eqn:Heqb.
   - (* x = x0 *)
     apply eqb_eq in Heqb as Heq.
     subst.
-    unfold upd.
+    unfold gsubst.
     rewrite update_eq.
     rewrite update_eq.
     reflexivity.
   - (* x <> x0 *)
     apply eqb_neq in Heqb as Hneq.
-    unfold upd.
+    unfold gsubst.
     rewrite update_neq; auto.
     rewrite update_neq; auto.
 Qed.
 
 (** ** Predicates *)
 Definition P_Term (t : Term) :=
-  forall Delta Gamma X K U T,
+  forall Delta Gamma X K U T Tn,
     (X |-> K; Delta) ,, Gamma |-+ t : T ->
     empty |-* U : K ->
-    Delta ,, (upd X U Gamma) |-+ <{ [[U / X] t }> : (substituteT X U T).
+    normalise (substituteT X U T) Tn ->
+    Delta ,, (gsubst X U Gamma) |-+ <{ [[U / X] t }> : Tn.
     
 Definition P_Binding (b : Binding) : Prop :=
   forall Delta Gamma X K U,
-    (X |-> K; Delta) ,, Gamma |-ok b ->
+    (X |-> K; Delta) ,, Gamma |-ok_b b ->
     empty |-* U : K ->
-    Delta ,, (upd X U Gamma) |-ok <{ [[U / X][b] b }>.
+    Delta ,, (gsubst X U Gamma) |-ok_b <{ [[U / X][b] b }>.
+
+#[export] Hint Unfold
+  P_Term
+  P_Binding
+  : core.
 
 Theorem substituteA_preserves_typing : 
   forall t, P_Term t.
-Proof. (*
+Proof with (eauto using substituteT_preserves_kinding with typing). 
   apply Term__ind with P_Binding.
-  - apply skip.
-  - (* Var *)
-    intros x. 
-    unfold P_Term. 
-    intros Delta Gamma X K U T Htyp Hkind.
-
-    inversion Htyp. subst.
-    simpl.
-
-    apply T_Var.
-    apply upd__substituteT.
-    assumption.
-
+  all: intros.
+  all: unfold P_Term.
+  all: try (intros Delta Gamma X K U T Tn Htyp__t Hkind__U Hnorm__Tn).
+  all: unfold P_Binding.
+  all: try (intros Delta Gamma X K U Htyp__b Hkind__U).
+  all: try (inversion Htyp__t; subst).
+  - admit.
+  - admit.
+  - simpl.
+    eapply T_Var.
+    + apply gsubst__substituteT.
+      apply H0.
+    + admit.
+  - simpl.
+    admit.
+  - simpl.
+    simpl in Hnorm__Tn.
+    inversion Hnorm__Tn.
     subst.
-    simpl.
-
-    apply T_Var.
-    apply upd__substituteT.
-    apply skip.
-
-  - (* TyAbs*) 
-    intros bX K t_body IH__t_body.
-    unfold P_Term.
-    intros Delta Gamma X L U T Htyp Hkind.
-
-    simpl.
-    destruct (X =? bX) eqn:Heqb.
-    + apply eqb_eq in Heqb as Heq.
-      subst.
-      simpl.
-      apply skip.
-    + apply eqb_neq in Heqb as Hneq.
-      apply T_TyAbs.
-
-    inversion Htyp. subst.
-    simpl.
-    destruct (X =? bX) eqn:Heqb.
-    + apply eqb_eq in Heqb as Heq.
-      subst.
-      simpl.
-      (*
-      unfold extendK in H4.
-      simpl in H4.
-      apply 
-
-      apply T_TyAbs.
-      unfold extendK.
-      simpl.
-      unfold P_Term in IH__t_body.
-      eapply IH__t_body.*)
-      apply skip.
-    + apply eqb_neq in Heqb as Hneq.
-      apply T_TyAbs.
-      eapply IH__t_body.
-      * simpl.
-        rewrite update_permute; auto.
-        apply H5. 
-      * apply Hkind.
-
-    + subst.
-    {
-
-    }
-  - (* LamAbs *)
-    intros bx T0 t_body IH__t_body.
-    unfold P_Term. 
-    intros Delta Gamma X L U T Htyp Hkind.
-
-    inversion Htyp. subst.
-    
-    simpl.
-    apply T_LamAbs.
-    + unfold P_Term in IH__t_body.
-      rewrite upd_absorbs_substituteT.
-      eapply IH__t_body; eauto.
-    + simpl.
-      eapply substituteT_preserves_kinding.
-      * eapply H6.
-      * assumption.
-  - (* Apply *) 
-    intros t1 IH__t1 t2 IH__t2.
-    unfold P_Term.
-    intros Delta Gamma X L U T Htyp Hkind.
-
-    inversion Htyp. subst.
-    
-    simpl.
-
-    eapply T_Apply.
-    + eapply IH__t1 in H3; eauto.
-    + eapply IH__t2; eauto.
-  - (* Constant *)
-    intros sv.
-    unfold P_Term.
-    intros Delta Gamma X L U T Htyp Hkind.
-
-    inversion Htyp. subst.
-
-    simpl.
-    eauto with typing.
-  - (* Builtin *)
-    intros d.
-    unfold P_Term.
-    intros Delta Gamma X L U T Htyp Hkind.
-
-    inversion Htyp. subst.
-
-    destruct d; try simpl; try apply T_Builtin; auto. 
-    destruct (X =? "a") eqn:Heqb.
-    + reflexivity.
-    + reflexivity.
-  
-  - (* TyInst *)
-    intros t_body IH__t_body V.
-    unfold P_Term.
-    intros Delta Gamma X L U T Htyp Hkind.
-
-    inversion Htyp. subst.
-    simpl.
-
-    assert (Delta ,, (upd X U Gamma) |-+ <{ [[U / X] t_body }>: (substituteT X U (Ty_Forall X0 K2 T1))) by eauto.
-    
-    simpl in H.
-    destruct (X =? X0) eqn:Heqb.
-    + apply eqb_eq in Heqb. subst.
-      eapply T_TyInst.
-      * apply H.
-      * eapply substituteT_preserves_kinding; eauto.
-      * apply skip. (* TODO *)
-      * apply skip.
-    + eapply T_TyInst.
-      * apply H.
-      * eapply substituteT_preserves_kinding; eauto.
-      * apply skip.
-      * apply skip. (* TODO *)
-  - (* Error *)
-    intros T0.
-    unfold P_Term.
-    intros Delta Gamma X L U T Htyp Hkind.
-
-    inversion Htyp. subst.
-  
-    apply T_Error.
-    eapply substituteT_preserves_kinding; eauto.
-  - (* IWrap *)
-    intros F0 T0 t0 IH__t0.
-    unfold P_Term.
-    intros Delta Gamma X L U T Htyp Hkind.
-    
-    inversion Htyp. subst.
-    simpl.
-
-    eapply T_IWrap.
-    + apply skip. (* TODO *)
-    + eauto.
-    + eapply substituteT_preserves_kinding; eauto.
-    + eapply substituteT_preserves_kinding; eauto.
-  - (* Unwrap *)
-    intros t0 IH__t0.
-    unfold P_Term.
-    intros Delta Gamma X L U T Htyp Hkind.
-    
-    inversion Htyp. subst.
-    simpl.*)
+    eapply T_LamAbs...
 Admitted.
