src/Language/PlutusIR/Semantics/TypeSafety/SubstitutionPreservesTyping/TermSubstitution.v
@@ -3,237 +3,22 @@ Import NamedTerm.
 Require Import PlutusCert.Language.PlutusIR.Semantics.Static.
 Require Import PlutusCert.Language.PlutusIR.Semantics.Dynamic.Substitution.
 
-Require Import Coq.Strings.String.
 Require Import Coq.Logic.FunctionalExtensionality.
 
-(*
-Lemma append_extendT_shadow : forall ctx' x T U ctx,
-    lookupT ctx' x = Datatypes.Some T ->
-    Implementations.append ctx' (x |T-> U; ctx) = Implementations.append ctx' ctx.
-Proof.
-  intros.
-  unfold Implementations.append.
-  apply cong_eq.
-  - reflexivity.
-  - apply functional_extensionality.
-    intros.
-    simpl.
-    destruct (lookupT ctx' x0) eqn:Hx0.
-    + reflexivity.
-    + assert (forall ctx' x x0, lookupT ctx' x = Datatypes.Some T -> lookupT ctx' x0 = None -> x <> x0). {
-        intros.
-        intros Hcon.
-        subst.
-        rewrite H0 in H1.
-        inversion H1.
-      }
-      remember (H0 _ _ _ H Hx0).
-      clear Heqn.
-      rewrite update_neq; auto.
-Qed.
-
-Lemma append_extendT_permute : forall ctx' x U ctx,
-    lookupT ctx' x = None ->
-    Implementations.append ctx' (x |T-> U; ctx) = (x |T-> U; Implementations.append ctx' ctx).
-Proof. 
-  intros.
-  unfold Implementations.append.
-  apply cong_eq.
-  - reflexivity.
-  - apply functional_extensionality.
-    intros.
-    simpl.
-    destruct (lookupT ctx' x0) eqn:Hx0.
-    + assert (forall ctx' x x0 T, lookupT ctx' x = Datatypes.Some T -> lookupT ctx' x0 = None -> x <> x0). {
-        intros.
-        intros Hcon.
-        subst.
-        rewrite H0 in H1.
-        inversion H1.
-      }
-      remember (H0 _ _ _ _ Hx0 H).
-      clear Heqn.
-      rewrite update_neq; auto.
-      rewrite Hx0.
-      reflexivity.
-    + destruct (x =? x0) eqn:Heqb.
-      * apply eqb_eq in Heqb as Heq.
-        subst.
-        rewrite update_eq.
-        rewrite update_eq.
-        reflexivity.
-      * apply eqb_neq in Heqb as Hneq.
-        rewrite update_neq; auto.
-        rewrite update_neq; auto.
-        rewrite Hx0.
-        reflexivity.
-Qed.
-
-
-Lemma binds_binds_bound_vars : forall a x,
-    List.In x (bvb a) ->
-    exists U, lookupT (binds a) x = Datatypes.Some U.
-Proof.
-  intros.
-  destruct a.
-  - simpl.
-    destruct (getName v =? x) eqn:Heqb.
-    + apply eqb_eq in Heqb as Heq.
-      subst.
-      exists (getTy v).
-      apply update_eq.
-    + apply eqb_neq in Heqb as Hneq.
-      simpl in H.
-      destruct v.
-      simpl in H.
-      destruct H.
-      * apply Hneq in H.
-        destruct H.
-      * destruct H.
-  - simpl in H.
-    destruct t.
-    inversion H.
-  - simpl.
-Admitted.
-
-Lemma mapbinds_binds_bound_vars : forall bs x,
-  List.In x (bvbs bs) ->
-  exists U, lookupT (flatten (List.map binds bs)) x = Datatypes.Some U.
-Proof.
-  induction bs.
-  - intros.
-    inversion H.
-  - intros.
-    unfold term_vars_bound_by_bindings in H.
-    simpl in H.
-    apply List.in_app_or in H.
-    destruct H.
-    + simpl.
-      unfold flatten.
-      simpl.
-      rewrite concat_append.
-      simpl. 
-      destruct (lookupT (Implementations.concat (List.rev (List.map binds bs))) x).
-      * exists t.
-        reflexivity.
-      * destruct (lookupT (binds a) x) eqn:Hlookup.
-        -- exists t.
-           reflexivity.
-        -- apply binds_binds_bound_vars in H.
-           destruct H. 
-           rewrite H in Hlookup.
-           inversion Hlookup.
-    + simpl.
-      unfold flatten.
-      simpl.
-      rewrite concat_append.
-      simpl.
-      destruct (lookupT (Implementations.concat (List.rev (List.map binds bs))) x) eqn:Hlookup.
-      * exists t.
-        reflexivity.
-      * apply IHbs in H.
-        destruct H.
-        unfold flatten in H.
-        rewrite H in Hlookup.
-        inversion Hlookup.
-Qed.
-
-Lemma binds_unbinds_unbound_vars : forall a x,
-    ~(List.In x (term_vars_bound_by_binding a)) ->
-    lookupT (binds a) x = None.
-Proof.
-  intros.
-  destruct a.
-  - simpl.
-    destruct (getName v =? x) eqn:Heqb.
-    + apply eqb_eq in Heqb as Heq.
-      subst.
-      destruct v.
-      exfalso.
-      apply H.
-      simpl.
-      left.
-      reflexivity.
-    + apply eqb_neq in Heqb as Hneq.
-      apply update_neq.
-      assumption.
-  - reflexivity.
-  - simpl.
-    destruct d.
-    simpl.
-    destruct (s =? x) eqn:Heqb.
-    + apply eqb_eq in Heqb as Heq.
-      subst.
-      exfalso.
-      apply H.
-      simpl.
-      destruct t.
-      simpl.
-      left.
-      reflexivity.
-    + apply eqb_neq in Heqb as Hneq.
-      rewrite update_neq; auto.
-      destruct  (lookupT
-      (List.fold_right Implementations.append emptyContext
-         (List.map
-            (fun x0 : binderTyname * Ty => fst x0 |T-> snd x0; emptyContext)
-            (List.map (constrBind (Datatype t l s l0)) l0))) x) eqn:E.
-      * exfalso.
-        apply H.
-        simpl.
-        destruct t.
-        simpl.
-        right.
-Admitted.
-
-Lemma mapbinds_unbinds_unbound_vars : forall bs x,
-    ~(List.In x (term_vars_bound_by_bindings bs)) ->
-    lookupT (flatten (List.map binds bs)) x = None.
-Proof.
-  induction bs.
-  - intros.
-    reflexivity.
-  - intros.
-    simpl.
-    unfold flatten.
-    simpl.
-    rewrite concat_append.
-    simpl.
-    destruct (lookupT (Implementations.concat (List.rev (List.map binds bs))) x) eqn:Hlookup.
-    + rewrite IHbs in Hlookup.
-      * symmetry in Hlookup.
-        assumption.
-      * intros Hcon.
-        apply H.
-        unfold term_vars_bound_by_bindings.
-        simpl.
-        apply List.in_or_app.
-        right.
-        assumption.
-    + destruct (lookupT (binds a) x) eqn:Hlookup'.
-      * rewrite binds_unbinds_unbound_vars in Hlookup'.
-        -- auto.
-        -- intros Hcon.
-           apply H.
-           unfold term_vars_bound_by_bindings.
-           simpl.
-           apply List.in_or_app.
-           left.
-           assumption.
-      * reflexivity.
-Qed. *)
 
 Definition P_Term (t : Term) :=
-  forall Delta Gamma x U v T,
+  forall Delta Gamma x U Un v T,
     Delta ,, (x |-> U; Gamma) |-+ t : T ->
-    empty ,, empty |-+ v : U ->
+    normalise U Un ->
+    empty ,, empty |-+ v : Un ->
     Delta ,, Gamma |-+ <{ [v / x] t }> : T.
 
 Definition P_Binding (b : Binding) : Prop :=
-  forall Delta Gamma x U v,
-    Delta ,, (x |-> U; Gamma) |-ok b ->
-    empty ,, empty |-+ v : U ->
-    Delta ,, Gamma |-ok <{ [v / x][b] b }> /\ 
+  forall Delta Gamma x U Un v,
+    Delta ,, (x |-> U; Gamma) |-ok_b b ->
+    normalise U Un ->
+    empty ,, empty |-+ v : Un ->
+    Delta ,, Gamma |-ok_b <{ [v / x][b] b }> /\ 
     binds_Delta b = binds_Delta <{ [v / x][b] b }> /\
     binds_Gamma b = binds_Gamma <{ [v / x][b] b}>.
 
@@ -242,228 +27,109 @@ Definition P_Binding (b : Binding) : Prop :=
   P_Binding
   : core.
 
-Lemma P_letnonrec : forall bs t Delta Gamma x U v T,
+Lemma P_letnonrec : forall bs t Delta Gamma x U Un v T,
     P_Term t ->
     Delta ,, (x |-> U; Gamma) |-+ (Let NonRec bs t) : T ->
-    empty ,, empty |-+ v : U ->
+    normalise U Un ->
+    empty ,, empty |-+ v : Un ->
     Util.ForallP P_Binding bs ->
     Delta ,, Gamma |-+ <{ [v / x] {Let NonRec bs t} }> : T /\ 
     List.map binds_Delta bs = List.map binds_Delta <{ [v / x][bnr] bs }> /\
     List.map binds_Gamma bs = List.map binds_Gamma <{ [v / x][bnr] bs }>.
-Proof.
+Proof with (eauto with typing).
   induction bs; intros.
   - simpl.
-    split.
-    + eapply T_Let.
-      * reflexivity.
-      * simpl; eauto.
-      * reflexivity.
-      * econstructor.
-      * simpl.
-        eapply H; eauto.
-        inversion H0. subst.
-        eauto.
-        apply skip.
-      
-    + auto.
-  - inversion H0. subst.
-    simpl.
-    destruct (List.existsb (eqb x) (bvb a)) eqn:Hexb.
-    + (* apply binds_binds_bound_vars in H6 as H15.
-      destruct H15 as [U' Hlu].
-      split.
-      * eapply T_Let.
-        -- reflexivity.
-        -- apply W_ConsB_NonRec.
-           ++ eapply Util.ForallP_hd in H2.
-              eapply H2; eauto.
-           ++ eapply Util.ForallP_hd in H2.
-              unfold P_Binding in H2.
-              assert (binds a = binds b') by (eapply H2; eauto).
-              rewrite <- H4.
-              erewrite append_extendT_shadow in H9; eauto.
-        -- eapply weakening; eauto. *)
+    split...
+    eapply T_Let...
+    + simpl.
+      eapply H...
+      inversion H0. subst.
+      simpl in H12.
+      simpl in H7.
+      inversion H7. subst.
+      eauto.
+    + inversion H0. subst...
+  - admit.
 Admitted.
 
-Lemma P_letrec : forall bs t Delta Gamma x U v T,
+Lemma P_letrec : forall bs t Delta Gamma x U Un v T,
     P_Term t ->
     Delta ,, (x |-> U; Gamma) |-+ (Let Rec bs t) : T ->
-    empty ,, empty |-+ v : U ->
+    normalise U Un ->
+    empty ,, empty |-+ v : Un ->
     Util.ForallP P_Binding bs ->
     Delta ,, Gamma |-+ <{ [v / x] {Let Rec bs t} }> : T /\ 
     List.map binds_Delta bs = List.map binds_Delta <{ [v / x][br] bs }> /\
     List.map binds_Gamma bs = List.map binds_Gamma <{ [v / x][br] bs}>.
-Proof. Admitted.
+Proof with (eauto with typing).
+  induction bs; intros.
+  - simpl.
+    split...
+    eapply T_LetRec...
+    + simpl.
+      eapply H...
+      inversion H0. subst.
+      simpl in H12.
+      simpl in H7.
+      inversion H7. subst.
+      eauto.
+    + inversion H0. subst...
+  - admit.
+Admitted.
 
 Lemma substitution_preserves_typing : 
   (forall t, P_Term t) /\ (forall b, P_Binding b).
-Proof.
+Proof with eauto.
   apply Term__multind with 
     (P := P_Term) 
     (Q := P_Binding).
   all: intros; autounfold; intros.
+  all: try solve [try (inversion H || inversion H0 || inversion H1); subst; eauto with typing].
   - destruct rec.
     + simpl.
       all: eapply P_letnonrec; eauto.
     + simpl.
       all: eapply P_letrec; eauto.
   - simpl.
-    destruct (x =? s) eqn:Heqb.
+    destruct (x =? s)%string eqn:Heqb.
     + apply eqb_eq in Heqb as Heq.
       subst.
       inversion H.
       subst.
-      rewrite update_eq in H2.
-      inversion H2. subst.
-      apply has_type__normal in H0 as H7.
-      eapply normalisation__stability in H7; eauto.
-      subst. 
-      eapply weakening_empty; eauto.
+      rewrite update_eq in H3.
+      inversion H3. subst.
+      assert (Un = T) by eauto using normalisation__deterministic.
+      subst.
+      eapply Typing.weakening_empty; eauto.
     + apply eqb_neq in Heqb as Hneq.
       inversion H. subst.
-      eapply T_Var.
-      * rewrite update_neq in H2; eauto.
-      * eassumption.
-  - (* TyAbs *) 
-    inversion H0. subst.
-    simpl.
-    apply T_TyAbs.
-    eapply H.
-    + eauto.
-    + eauto.
+      eapply T_Var...
+      rewrite update_neq in H3...
   - (* LamAbs *)
     inversion H0. subst.
     simpl.
-    destruct (x =? s) eqn:Heqb.
+    destruct (x =? s)%string eqn:Heqb.
     + apply eqb_eq in Heqb as Heq. 
       subst.
-      apply T_LamAbs.
-      * assumption.
-      * eauto.
-      * rewrite update_shadow in H10.
-        eauto.
+      apply T_LamAbs...
+      rewrite update_shadow in H11...
     + apply eqb_neq in Heqb as Hneq.
-      apply T_LamAbs.
-      * eauto.
-      * eauto.
-      * eapply H.
-      -- rewrite update_permute; auto.
-         apply H10.
-      -- eassumption.
-  - (* Apply *)
-    inversion H1. subst.
-    simpl.
-    eapply T_Apply.
-    + eapply H.
-      * eassumption.
-      * eassumption.
-    + eapply H0.
-      * eassumption.
-      * eassumption.
-  - (* Constant *)
-    inversion H. subst.
-    simpl.
-    apply T_Constant.
-  - (* Builtin *) 
-    inversion H. subst.
-    simpl.
-    apply T_Builtin.
-    reflexivity.
-  - (* TyInst *)
-    inversion H0. subst.
-    simpl.
-    eapply T_TyInst.
-    + eapply H.
-      * eassumption.
-      * eassumption.
-    + eauto.
-    + eassumption.
-    + eassumption.
-  - (* Error *)
-    inversion H. subst.
-    simpl.
-    apply T_Error.
-    eauto.
-    eauto.
-  - (* IWrap *)
-    inversion H0. subst.
-    simpl.
-    eapply T_IWrap.
-    + eassumption.
-    + eapply H.
-      * eassumption.
-      * eassumption.
-    + eauto.
-    + eauto.
-    + eauto.
-    + eauto.
-  - (* Unwrap *)
-    inversion H0. subst.
-    simpl.
-    eapply T_Unwrap.
-    + eapply H.
-      * eassumption.
-      * eassumption.
-    + eauto.
-    + eassumption.
+      apply T_LamAbs...
+      rewrite update_permute in H11...
+Admitted.
 
-  - (* ExtBuiltin *)
-    inversion H0. subst.
-    simpl.
-    erewrite <- List.map_length.
-    eapply T_ExtBuiltin; eauto.
-    + rewrite List.map_length. auto.
-    + intros.
-      destruct p.
-      simpl.
-      apply List.in_combine_l in H2 as H15.
-      apply List.in_combine_r in H2 as H16.
-      eapply List.in_map_iff in H15 as H17.
-      destruct H17. 
-      destruct H3.
-      subst.
-
-      apply skip.
-
-  - (* TermBind *)
-    inversion H0. subst.
-    simpl.
-    split.
-    + apply W_Term.
-      * eauto.
-      * eapply H.
-        -- eassumption.
-        -- eassumption.
-    + auto. 
-  - (* TypeBind *)
-    inversion H. subst.
-    simpl.
-    split. 
-    + apply W_Type.
-      eauto.
-    + auto.
-  - (* DatatypeBind *)
-    inversion H. subst.
-    split.
-    + simpl.
-      eapply W_Data.
-      * reflexivity.
-      * reflexivity.
-      * intros.
-        eauto.
-    + auto.
-Qed. 
-
-Corollary substitution_preserves_typing__Term : forall t Delta Gamma x U v T,
+Corollary substitution_preserves_typing__Term : forall t Delta Gamma x U Un v T,
     Delta ,, (x |-> U; Gamma)  |-+ t : T ->
-    empty ,, empty |-+ v : U ->
+    normalise U Un ->
+    empty ,, empty |-+ v : Un ->
     Delta ,, Gamma |-+ <{ [v / x] t }> : T.
 Proof. apply substitution_preserves_typing. Qed.
 
-Corollary substitution_preserves_typing__Binding : forall b Delta Gamma x U v,
-    Delta ,, (x |-> U; Gamma) |-ok b ->
-    empty ,, empty |-+ v : U ->
-    Delta ,, Gamma |-ok <{ [v / x][b] b }> /\ 
+Corollary substitution_preserves_typing__Binding : forall b Delta Gamma x U Un v,
+    Delta ,, (x |-> U; Gamma) |-ok_b b ->
+    normalise U Un ->
+    empty ,, empty |-+ v : Un ->
+    Delta ,, Gamma |-ok_b <{ [v / x][b] b }> /\ 
     binds_Delta b = binds_Delta <{ [v / x][b] b }> /\
     binds_Gamma b = binds_Gamma <{ [v / x][b] b }>.
 Proof. apply substitution_preserves_typing. Qed.
