src/Language/PlutusIR/Semantics/Dynamic/Bigstep/Deterministic.v
@@ -1,6 +1,9 @@
 Require Import PlutusCert.Language.PlutusIR.
 Import NamedTerm.
+
 Require Import PlutusCert.Language.PlutusIR.Semantics.Dynamic.Bigstep.
+Require Import PlutusCert.Language.PlutusIR.Semantics.Dynamic.Bigstep.EvalToValue.
+Require Import PlutusCert.Language.PlutusIR.Semantics.Dynamic.Bigstep.EvalValue.
 
 (** * [eval] is deterministic *)
 
@@ -29,526 +32,156 @@ Definition P_eval x y1 (j1 : nat) :=
 
 Definition P_eval_bindings_nonrec x y1 (j1 : nat) :=
   forall y2 j2,
-    eval_bindings_nonrec x y2 j2 ->
+    x =[j2]=>nr y2 ->
     y1 = y2 /\ j1 = j2.
 
 Definition P_eval_bindings_rec bs0 x y1 (j1 : nat) :=
   forall y2 j2,
-    eval_bindings_rec bs0 x y2 j2->
+    x =[j2]=>r y2 WITH bs0 ->
     y1 = y2 /\ j1 = j2.
+
+#[export] Hint Unfold
+  P_eval
+  P_eval_bindings_nonrec
+  P_eval_bindings_rec
+  : core.
+
+Ltac unfold_predicates :=
+  match goal with
+  | H : P_eval ?t ?v ?j |- ?P =>
+      unfold P_eval in H; unfold_predicates
+  | H : P_eval_bindings_nonrec ?t ?v ?j |- ?P =>
+      unfold P_eval_bindings_nonrec in H; unfold_predicates
+  | H : P_eval_bindings_rec ?bs0 ?t ?v ?j |- ?P =>
+      unfold P_eval_bindings_rec in H; unfold_predicates
+  | |- _ => idtac
+  end.
+
+Ltac e :=
+  let y2 := fresh "y2" in
+  let j2 := fresh "j2" in
+  let H4 := fresh "H" in
+  let H5 := fresh "H" in
+  match goal with
+  | H1 : forall y2 j2, ?x =[j2]=> y2 -> ?y1 = y2 /\ ?j1 = j2, 
+    H2 : ?x =[?j1]=> ?v1, 
+    H3 : ?x =[?j3]=> ?v3
+      |- ?v = ?v' /\ ?j = ?j' =>
+    eapply H1 in H3; eauto; destruct H3 as [H4 H5]; try (inversion H4); subst
+  | H1 : forall y2 j2, ?x =[j2]=>nr y2 -> ?y1 = y2 /\ ?j1 = j2, 
+    H2 : ?x =[?j1]=>nr ?v1, 
+    H3 : ?x =[?j3]=>nr ?v3
+      |- ?v = ?v' /\ ?j = ?j' =>
+    eapply H1 in H3; eauto; destruct H3 as [H4 H5]; try (inversion H4); subst
+  | H1 : forall y2 j2, ?x =[j2]=>r y2 WITH ?bs0 -> ?y1 = y2 /\ ?j1 = j2, 
+    H2 : ?x =[?j1]=>r ?v1 WITH ?bs0, 
+    H3 : ?x =[?j3]=>r ?v3 WITH ?bs0
+      |- ?v = ?v' /\ ?j = ?j' =>
+    eapply H1 in H3; eauto; destruct H3 as [H4 H5]; try (inversion H4); subst
+  end. 
+
+Ltac f :=
+  match goal with
+  | H : ~ is_error (Error ?T) |- ?P =>
+      exfalso; apply H; constructor
+  end.
+
+Ltac g :=
+  match goal with
+  | H : neutral ?t |- ?P =>
+      try solve [inversion H]
+  | H : neutral_value ?n ?t |- ?P =>
+      try solve [inversion H]
+  end.
+
+Ltac solf :=
+  try solve [repeat (e || f || g || eauto)].
+
+Ltac solf' :=
+  repeat (e || f || g || eauto).
+
+Ltac h n :=
+  match goal with
+  | H : ?t =[?j]=> ?v |- ?P =>
+      inversion H; clear H; subst; 
+      try solve [
+        solf' || exfalso; eauto
+      ];
+      match n with
+      | S (S ?n') => try (h (S n'))
+      end
+  end.
+
+Axiom skip : forall P, P.
 
 (** ** The main result *)
 Theorem eval__deterministic : forall x y1 j1,
   x =[j1]=> y1 ->
   P_eval x y1 j1.
-Proof.
+Proof with eauto.
   apply eval__ind with (P := P_eval) (P0 := P_eval_bindings_nonrec) (P1 := P_eval_bindings_rec).
-  - (* E_Let *)
-    intros. unfold P_eval. intros.
-    inversion H1. subst.
-    eapply H0.
-    eassumption.
-  - (* E_LetRec *)
-    intros. unfold P_eval. intros.
-    inversion H1. subst.
-    eapply H0.
-    eassumption.
-  - (* E_TyAbs *)
-    intros. unfold P_eval. intros.
-    inversion H. subst.
-    split; auto.
-  - (* E_LamAbs *)
-    intros. unfold P_eval. intros.
-    inversion H. subst.
-    split; auto.
-  - (* E_Apply *)
-    intros. unfold P_eval. intros.
-    inversion H5.
-    + (* E_Apply *)
-      subst.
-
-      assert (LamAbs x T t0 = LamAbs x0 T0 t5). {
-        eapply H0. eassumption.
-      }
-      inversion H6. subst.
-      assert (v2 = v1). {
-        eapply H2. eassumption.
-      }
-      subst.
-
-      split.
-      * eapply H4. 
-        eassumption.
-      * assert (j1 = j4). {
-          eapply H0. eassumption.
-        }
-        assert (j2 = j5). {
-          eapply H2. eassumption.
-        }
-        assert (j0 = j6). {
-          eapply H4. eassumption.
-        } 
-        subst.
-        reflexivity.
-    + (* E_ApplyExtBuiltin *)
-      subst.
-      assert (LamAbs x T t0 = ExtBuiltin f args). {
-        eapply H0. eassumption.
-      }
-      inversion H6.
-    + (* E_IfCondition*)
-      subst.
-      assert (LamAbs x T t0 = TyInst (Builtin IfThenElse) T0). {
-        eapply H0. eassumption.
-      }
-      inversion H6.
-    + (* E_IfThenBranch *)
-      subst.
-      assert (LamAbs x T t0 = Apply (TyInst (Builtin IfThenElse) T0) (Constant (Some (ValueOf DefaultUniBool cond)))). {
-        eapply H0. eassumption.
-      }
-      inversion H6.
-    + (* E_IfTrue *)
-      subst.
-      assert (LamAbs x T t0 = Apply (Apply (TyInst (Builtin IfThenElse) T0) (Constant (Some (ValueOf DefaultUniBool true)))) t_t). {
-        eapply H0. eassumption.
-      }
-      inversion H6.
-    + (* E_IfFalse *)
-      subst.
-      assert (LamAbs x T t0 = Apply (Apply (TyInst (Builtin IfThenElse) T0) (Constant (Some (ValueOf DefaultUniBool false)))) t_t). {
-        eapply H0. eassumption.
-      }
-      inversion H6.
-  - (* E_Constant *)
-    intros. unfold P_eval. intros.
-    inversion H. subst.
-    auto.
-  - (* E_Builtin *)
-    intros. unfold P_eval. intros.
-    inversion H0.
-    + subst.
-      auto.
-    + subst.
-      exfalso.
-      eauto.
-  - (* E_ExtBuiltinPartiallyApplied *)
-    intros. unfold P_eval. intros.
-    inversion H0. all: subst.
-    + auto.
-    + rewrite H3 in H.
-      apply PeanoNat.Nat.lt_irrefl in H.
-      exfalso.
-      auto.
-  - (* E_ExtBuiltinFullyApplied *)
-    intros. unfold P_eval. intros.
-    inversion H1. all: subst.
-    + rewrite H in H6.
-      apply PeanoNat.Nat.lt_irrefl in H6.
-      exfalso. auto.
-    + rewrite H0 in H7.
-      inversion H7. subst. 
-      auto.
-  - (* E_ApplyExtBuiltin *)
-    intros. unfold P_eval. intros.
-    inversion H5. subst.
-    + (* E_Apply *) 
-      subst.
-      assert (ExtBuiltin f args = LamAbs x T t4). {
-        eapply H0. eassumption.
-      }
-      inversion H6.
-    + (* E_ApplyExtBuiltin *)
-      subst.
-      assert (ExtBuiltin f args = ExtBuiltin f0 args0 /\ j1 = j4). {
-        eapply H0. eassumption.
-      }
-      destruct H6.
-      inversion H6.
-      subst.
-      assert (v2 = v1 /\ j2 = j5). {
-        eapply H2. eassumption.
-      }
-      destruct H7.
-      subst.
-      assert (v0 = y2 /\ j3 = j6). {
-        eapply H4. assumption.
-      }
-      destruct H7. subst.
-      auto.
-(*
-    + (* E_IfCondition*)
-      subst.
-      assert (v1 = TyInst (Builtin IfThenElse) T). {
-        eapply H0. eassumption.
-      }
-      subst.
-      inversion H4.
-    + (* E_IfThenBranch *)
-      subst.
-      assert (v1 = Apply (TyInst (Builtin IfThenElse) T) (Constant (Some (ValueOf DefaultUniBool cond)))). {
-        eapply H0. eassumption.
-      }
-      subst.
-      inversion H4.
-    + (* E_IfTrue *)
-      subst.
-      assert (v1 = Apply (Apply (TyInst (Builtin IfThenElse) T) (Constant (Some (ValueOf DefaultUniBool true)))) t_t). {
-        eapply H0. eassumption.
-      }
-      subst.
-      inversion H4.
-    + (* E_IfFalse *)
-      subst.
-      assert (v1 = Apply (Apply (TyInst (Builtin IfThenElse) T) (Constant (Some (ValueOf DefaultUniBool false)))) t_t). {
-        eapply H0. eassumption.
-      }
-      subst.
-      inversion H4.
-  - (* E_ApplyBuiltin2 *)
-    intros. unfold P_eval. intros.
-    inversion H6. subst.
-    + (* E_Apply *) 
-      subst.
-      assert (v1 = LamAbs x T t4). {
-        eapply H0. eassumption.
-      }
-      subst.
-      inversion H1.
-    + (* E_ApplyBuiltin1 *)
-      subst.
-      assert (v1 = v3). {
-        eapply H0. eassumption.
-      }
-      subst.
-      assert (v2 = v4). {
-        eapply H3. eassumption.
-      }
-      subst.
-      apply H4 in H14.
-      destruct H14.
-    + (* E_ApplyBuiltin2 *)
-      subst.
-      assert (v1 = v3). {
-        eapply H0. eassumption.
-      }
-      subst.
-      assert (v2 = v4). {
-        eapply H3. eassumption.
-      }
-      subst. 
-      rewrite H5 in H15. 
-      inversion H15. 
-      subst. 
-      reflexivity.
-    + (* E_IfCondition*)
-      subst.
-      assert (v1 = TyInst (Builtin IfThenElse) T). {
-        eapply H0. eassumption.
-      }
-      subst.
-      inversion H1.
-    + (* E_IfThenBranch *)
-      subst.
-      assert (v1 = Apply (TyInst (Builtin IfThenElse) T) (Constant (Some (ValueOf DefaultUniBool cond)))). {
-        eapply H0. eassumption.
-      }
-      subst.
-      inversion H1.
-    + (* E_IfTrue *)
-      subst.
-      assert (v1 = Apply (Apply (TyInst (Builtin IfThenElse) T) (Constant (Some (ValueOf DefaultUniBool true)))) t_t). {
-        eapply H0. eassumption.
-      }
-      subst.
-      inversion H1.
-    + (* E_IfFalse *)
-      subst.
-      assert (v1 = Apply (Apply (TyInst (Builtin IfThenElse) T) (Constant (Some (ValueOf DefaultUniBool false)))) t_t). {
-        eapply H0. eassumption.
-      }
-      subst.
-      inversion H1.
-  - (* E_IfTyInst *)
-    intros. unfold P_eval. intros.
-    inversion H1.
-    + (* E_IfTyInst *)
-      reflexivity.
-    + (* E_TyInst *)  
-      subst.
-      assert (Builtin IfThenElse = TyAbs X j t2). {
-        eapply H0. eassumption.
-      }
-      inversion H2.
-  - (* E_IfCondition *)
-    intros. unfold P_eval. intros.
-    inversion H3.
-    + (* E_Apply *) 
-      subst.
-      assert (TyInst (Builtin IfThenElse) T = LamAbs x T0 t0). {
-        eapply H0. eassumption.
-      }
-      inversion H4.
-    + (* E_ApplyBuiltin1 *)
-      assert (TyInst (Builtin IfThenElse) T = v1). {
-        eapply H0. eassumption.
-      }
-      subst.
-      inversion H7.
-    + (* E_ApplyBuiltin2 *)
-      subst.
-      assert (TyInst (Builtin IfThenElse) T = v1). {
-        eapply H0. eassumption.
-      }
-      subst.
-      inversion H7.
-    + (* E_IfCondition*)
-      subst.
-      f_equal.
-      * eapply H0. eassumption.
-      * eapply H2. eassumption.
-    + (* E_IfThenBranch *)
-      subst.
-      assert (TyInst (name := Strings.String.string) (binderName := Strings.String.string) (Builtin IfThenElse) T = Apply (TyInst (Builtin IfThenElse) T0) (Constant (Some (ValueOf DefaultUniBool cond0)))). {
-        eapply H0. eassumption.
-      }
-      inversion H4.
-    + (* E_IfTrue *)
-      subst.
-      assert (TyInst (name := Strings.String.string) (binderName := Strings.String.string) (Builtin IfThenElse) T = Apply (Apply (TyInst (Builtin IfThenElse) T0) (Constant (Some (ValueOf DefaultUniBool true)))) t_t). {
-        eapply H0. eassumption.
-      }
-      subst.
-      inversion H4.
-    + (* E_IfFalse *)
-      subst.
-      assert (TyInst (name := Strings.String.string) (binderName := Strings.String.string) (Builtin IfThenElse) T = Apply (Apply (TyInst (Builtin IfThenElse) T0) (Constant (Some (ValueOf DefaultUniBool false)))) t_t). {
-        eapply H0. eassumption.
-      }
-      subst.
-      inversion H4.
-  - (* E_IfThenBranch *)
-    intros. unfold P_eval. intros.
-    inversion H1.
-    + (* E_Apply *) 
-      subst.
-      assert (Apply (TyInst (Builtin IfThenElse) T) (Constant (Some (ValueOf DefaultUniBool cond))) = LamAbs x T0 t0). {
-        eapply H0. eassumption.
-      }
-      inversion H2.
-    + (* E_ApplyBuiltin1 *)
-      assert (Apply (TyInst (Builtin IfThenElse) T) (Constant (Some (ValueOf DefaultUniBool cond))) = v1). {
-        eapply H0. eassumption.
-      }
-      subst.
-      inversion H9.
-    + (* E_ApplyBuiltin2 *)
-      subst.
-      assert (Apply (TyInst (Builtin IfThenElse) T) (Constant (Some (ValueOf DefaultUniBool cond))) = v1). {
-        eapply H0. eassumption.
-      }
-      subst.
-      inversion H5.
-    + (* E_IfCondition*)
-      subst.
-      assert (Apply (name := Strings.String.string) (binderName := Strings.String.string) (TyInst (Builtin IfThenElse) T) (Constant (Some (ValueOf DefaultUniBool cond))) = (TyInst (Builtin IfThenElse) T0)). {
-        eapply H0. eassumption.
-      }
-      inversion H2.
-    + (* E_IfThenBranch *)
-      subst.
-      f_equal.
-      eapply H0. eassumption.
-    + (* E_IfTrue *)
-      assert (Apply (name := Strings.String.string) (binderName := Strings.String.string) (TyInst (Builtin IfThenElse) T) (Constant (Some (ValueOf DefaultUniBool cond))) = Apply (Apply (TyInst (Builtin IfThenElse) T0) (Constant (Some (ValueOf DefaultUniBool true)))) t_t0). {
-        eapply H0. eassumption.
-      }
-      subst.
-      inversion H8.
-    + (* E_IfFalse *)
-      subst.
-      assert (Apply (name := Strings.String.string) (binderName := Strings.String.string) (TyInst (Builtin IfThenElse) T) (Constant (Some (ValueOf DefaultUniBool cond))) = Apply (Apply (TyInst (Builtin IfThenElse) T0) (Constant (Some (ValueOf DefaultUniBool false)))) t_t0). {
-        eapply H0. eassumption.
-      }
-      inversion H2.
-  - (* E_IfTrue *)
-    intros. unfold P_eval. intros.
-    inversion H3.
-    + (* E_Apply *) 
-      subst.
-      assert (Apply (Apply (TyInst (Builtin IfThenElse) T) (Constant (Some (ValueOf DefaultUniBool true)))) t_t = LamAbs x T0 t0). {
-        eapply H0. eassumption.
-      }
-      inversion H4.
-    + (* E_ApplyBuiltin1 *)
-      assert (Apply (Apply (TyInst (Builtin IfThenElse) T) (Constant (Some (ValueOf DefaultUniBool true)))) t_t = v1). {
-        eapply H0. eassumption.
-      }
-      subst.
-      inversion H11.
-    + (* E_ApplyBuiltin2 *)
-      subst.
-      assert (Apply (Apply (TyInst (Builtin IfThenElse) T) (Constant (Some (ValueOf DefaultUniBool true)))) t_t = v1). {
-        eapply H0. eassumption.
-      }
-      subst.
-      inversion H7.
-    + (* E_IfCondition*)
-      subst.
-      assert (Apply (Apply (TyInst (Builtin IfThenElse) T) (Constant (Some (ValueOf DefaultUniBool true)))) t_t = (TyInst (Builtin IfThenElse) T0)). {
-        eapply H0. eassumption.
-      }
-      inversion H4.
-    + (* E_IfThenBranch *)
-      subst.
-      assert (Apply (Apply (TyInst (Builtin IfThenElse) T) (Constant (Some (ValueOf DefaultUniBool true)))) t_t = Apply (TyInst (Builtin IfThenElse) T0) (Constant (Some (ValueOf DefaultUniBool cond)))). {
-        eapply H0. eassumption.
-      }
-      inversion H4.
-    + (* E_IfTrue *)
-      subst.
-      assert (Apply (Apply (TyInst (Builtin IfThenElse) T) (Constant (Some (ValueOf DefaultUniBool true)))) t_t = Apply (Apply (TyInst (Builtin IfThenElse) T0) (Constant (Some (ValueOf DefaultUniBool true)))) t_t0). {
-        eapply H0. eassumption.
-      }
-      inversion H4.
-      subst.
-      eapply H2.
-      eassumption.
-    + (* E_IfFalse *)
-      subst.
-      assert (Apply (Apply (TyInst (Builtin IfThenElse) T) (Constant (Some (ValueOf DefaultUniBool true)))) t_t = Apply (Apply (TyInst (Builtin IfThenElse) T0) (Constant (Some (ValueOf DefaultUniBool false)))) t_t0). {
-        eapply H0. eassumption.
-      }
-      apply compare_IfThenElse_conditions in H4.
-      discriminate.
-  - (* E_IfFalse *)
-    intros. unfold P_eval. intros.
-    inversion H3.
-    + (* E_Apply *) 
-      subst.
-      assert (Apply (Apply (TyInst (Builtin IfThenElse) T) (Constant (Some (ValueOf DefaultUniBool false)))) t_t = LamAbs x T0 t0). {
-        eapply H0. eassumption.
-      }
-      inversion H4.
-    + (* E_ApplyBuiltin1 *)
-      assert (Apply (Apply (TyInst (Builtin IfThenElse) T) (Constant (Some (ValueOf DefaultUniBool false)))) t_t = v1). {
-        eapply H0. eassumption.
-      }
-      subst.
-      inversion H11.
-    + (* E_ApplyBuiltin2 *)
-      subst.
-      assert (Apply (Apply (TyInst (Builtin IfThenElse) T) (Constant (Some (ValueOf DefaultUniBool false)))) t_t = v1). {
-        eapply H0. eassumption.
-      }
-      subst.
-      inversion H7.
-    + (* E_IfCondition*)
-      subst.
-      assert (Apply (Apply (TyInst (Builtin IfThenElse) T) (Constant (Some (ValueOf DefaultUniBool false)))) t_t = (TyInst (Builtin IfThenElse) T0)). {
-        eapply H0. eassumption.
-      }
-      inversion H4.
-    + (* E_IfThenBranch *)
-      subst.
-      assert (Apply (Apply (TyInst (Builtin IfThenElse) T) (Constant (Some (ValueOf DefaultUniBool false)))) t_t = Apply (TyInst (Builtin IfThenElse) T0) (Constant (Some (ValueOf DefaultUniBool cond)))). {
-        eapply H0. eassumption.
-      }
-      inversion H4.
-    + (* E_IfTrue *)
-      subst.
-      assert (Apply (Apply (TyInst (Builtin IfThenElse) T) (Constant (Some (ValueOf DefaultUniBool false)))) t_t = Apply (Apply (TyInst (Builtin IfThenElse) T0) (Constant (Some (ValueOf DefaultUniBool true)))) t_t0). {
-        eapply H0. eassumption.
-      }
-      apply compare_IfThenElse_conditions in H4.
-      discriminate.
-    + (* E_IfFalse *)
-      subst.
-      assert (Apply (Apply (TyInst (Builtin IfThenElse) T) (Constant (Some (ValueOf DefaultUniBool false)))) t_t = Apply (Apply (TyInst (Builtin IfThenElse) T0) (Constant (Some (ValueOf DefaultUniBool false)))) t_t0). {
-        eapply H0. eassumption.
-      }
-      inversion H4.
-      subst.
-      eapply H2.
-      eassumption.
-  - (* E_TyInst *)
-    intros. unfold P_eval. intros.
-    inversion H4.
-    + (* E_IfTyInst *)
-      subst.
-      assert (TyAbs X j t0 = Builtin IfThenElse). {
-        eapply H0. eassumption.
-      }
-      inversion H5.
-    + (* E_TyInst *)
-      subst.
-      assert (TyAbs X j t0 = TyAbs X0 j0 t3). {
-        eapply H0. eassumption.
-      }
-      inversion H5. subst.
-      assert (t0' = t0'0). {
-        apply annotsubst__deterministic with X0 T2 t3; auto.
-      }
-      subst.
-      eapply H3.
-      eassumption.
-  - (* E_Error *)
-    intros. unfold P_eval. intros.
-    inversion H. subst.
-    reflexivity.
-  - (* E_IWrap *)
-    intros. unfold P_eval. intros.
-    inversion H1. subst.
-    f_equal.
-    eapply H0.
-    eassumption.
-  - (* E_Unwrap *)
-    intros. unfold P_eval. intros.
-    inversion H1. subst.
-    assert (IWrap F T v0 = IWrap F0 T0 y2). {
-      eapply H0. eassumption.  
-    }
-    inversion H2. subst.
-    reflexivity.
-  
-  - (* E_NilB_NonRec  *)
-    intros. unfold P_eval_bindings_nonrec. intros.
-    inversion H1. subst.
-    eapply H0. eassumption.
-  - (* E_ConsB_NonRec *)
-    intros. unfold P_eval_bindings_nonrec. intros.
-    inversion H4. subst.
-    assert (vb = vb0). {
-      eapply H0. eassumption.
-    }
-    subst.
-    assert (Let NonRec bs' t' = Let NonRec bs'0 t'0). {
-      apply substitute__deterministic in H1.
-      apply H1 in H14.
-      assumption.
-    }
-    inversion H5. 
-    subst.
-    eapply H3.
-    eassumption.
-  
-  - (* E_NilB_Rec *)
-    intros. unfold P_eval_bindings_rec. intros.
-    inversion H1. subst.
-    eapply H0.
-    eassumption.
-  - (* E_ConsB_Rec *)
-    intros. unfold P_eval_bindings_rec. intros.
-    inversion H2. subst.
-    assert (Let Rec bs' t' = Let Rec bs'0 t'0). {
-      apply substitute__deterministic in H.
-      apply H in H12.
-      assumption.
-    }
-    inversion H3. 
-    subst.
-    eapply H1.
-    eassumption.
-Qed.
-*)
+  all: intros; autounfold.
+  all: intros y5 j5 Hev.
+  all: unfold_predicates.
+  all: try solve [inversion Hev; subst; solf].
+  - inversion Hev; subst. 
+    all: try solve[solf].
+    + inversion H10. subst.
+      apply eval_value in H12.
+      autounfold in H12.
+      e.
+      inversion H10. subst.
+      inversion H15.
+    + inversion H8.
+      subst.
+      eapply fully_applied_neutral__subsumes__neutral_value in H13...
+      eapply eval_value in H13 as H14.
+      autounfold in H14.
+      e.
+      g.
+    + inversion H.
+      * subst. inversion H9.
+        -- subst. inversion H13.
+           ++ subst. inversion H17.
+           ++ subst. inversion H18.
+              ** subst. inversion H20.
+                 subst. exfalso...
+              ** subst. inversion H20.
+                 subst. exfalso...
+           ++ subst. inversion H17.
+              subst. inversion H18.
+              subst. exfalso...
+        -- subst. inversion H14.
+           ++ subst. inversion H19.
+           ++ subst. inversion H22.
+              subst. inversion H19.
+              subst. exfalso...
+           ++ subst. inversion H20.
+              ** subst. inversion H22.
+                 subst. exfalso...
+              ** subst. inversion H22.
+                 subst. exfalso...
+           ++ subst. inversion H19.
+              subst. inversion H20.
+              subst. exfalso...
+           ++ subst. inversion H16.
+              subst. inversion H19.
+              subst. exfalso...
+           ++ subst. inversion H16.
+        -- subst. inversion H13.
+           subst. inversion H19.
+           subst. inversion H16.
+           subst. exfalso...
+        -- subst.
+           inversion H13.
+           ++ subst. inversion H14.
+           ++ subst. inversion H16.
+              ** subst. exfalso... 
+              ** subst. inversion H18.
+                 subst. exfalso...
+           ++ subst. inversion H19.
+      * admit.
+      * admit.
+      * admit.
+    +  admit.
 Admitted.
