src/Language/PlutusIR/Semantics/Dynamic/Bigstep/Examples/IfThenElse.v
@@ -15,26 +15,20 @@ Definition int_and_int_to_int : Ty := Ty_Fun Ty_int (Ty_Fun Ty_int Ty_int).
 
 Example test_ifThenElse : forall x y, exists k,
   Apply (LamAbs x int_and_int_to_int (Apply (Apply (Var x) (constInt 17)) (constInt 3))) (Apply (TyInst (Apply (LamAbs y Ty_int (Builtin IfThenElse)) (constInt 666)) (Ty_Builtin (Some (TypeIn DefaultUniInteger)))) (Constant (Some (ValueOf DefaultUniBool true)))) =[k]=> constInt 17.
-Proof.
+Proof with eauto.
+  unfold constInt.
   intros.
   eexists.
-  eapply E_Apply.
-  - apply E_LamAbs.
-  - eapply E_IfCondition.
-    + eapply E_IfTyInst. 
-      eapply E_Apply.
-      * apply E_LamAbs.
-      * apply E_Constant.
-      * simpl. 
-        apply E_If.
-    + apply E_Constant.
-  - simpl.
-    rewrite eqb_refl.
-    eapply E_IfTrue.
-    + apply E_IfThenBranch.
-      * apply E_IfCondition.
-        -- apply E_IfTyInst.
-           apply E_If.
-        -- apply E_Constant.
-    + apply E_Constant.
+  eapply E_Apply... { 
+    eapply E_IfCondition...
+    eapply E_IfTyInst...
+    eapply E_Apply...
+    intros Hcon.
+    inversion Hcon.
+  } {
+    intros Hcon.
+    inversion Hcon.
+  }
+  simpl.
+  rewrite eqb_refl...
 Qed.
