src/Language/PlutusIR/Semantics/Dynamic/BuiltinMeanings.v
@@ -54,6 +54,17 @@ Definition constUnit (a : unit) : Term := Constant (Some (ValueOf DefaultUniUnit
 Definition take (x : Z) (s : string) : string := substring 0 (Z.to_nat x) s.
 Definition drop (x : Z) (s : string) : string := substring (Z.to_nat x) (length s) s.
 
+#[export] Hint Unfold
+  constInt
+  constBool
+  constBS
+  constChar
+  constString
+  constUnit
+  take
+  drop
+  : core.
+
 (** Computes results of fully applied default functions where possible.
     
     Note that not all default functions have sensible implementations, such
@@ -63,159 +74,201 @@ Definition compute_defaultfun (t : Term) : option Term :=
   match t with
   (** Binary operators on integers *)
   (* AddInteger *)
-  | ExtBuiltin AddInteger 
-      [ Constant (@Some _ DefaultUniInteger (ValueOf _ y)) 
-      ; Constant (@Some _ DefaultUniInteger (ValueOf _ x))
-      ] 
-      => Datatypes.Some (constInt (x + y))
+  | (Apply 
+      (Apply 
+        (Builtin AddInteger) 
+        (Constant (@Some _ DefaultUniInteger (ValueOf _ x)))
+      ) 
+      (Constant (@Some _ DefaultUniInteger (ValueOf _  y)))
+    ) => Datatypes.Some (constInt (x + y))
   (* SubtractInteger *)
-  | ExtBuiltin SubtractInteger 
-      [ Constant (@Some _ DefaultUniInteger (ValueOf _ y)) 
-      ; Constant (@Some _ DefaultUniInteger (ValueOf _ x))
-      ] 
-      => Datatypes.Some (constInt (x - y))
+  | (Apply 
+      (Apply 
+        (Builtin SubtractInteger) 
+        (Constant (@Some _ DefaultUniInteger (ValueOf _ x)))
+      ) 
+      (Constant (@Some _ DefaultUniInteger (ValueOf _ y)))
+    ) => Datatypes.Some (constInt (x - y))
   (* MultiplyInteger *)
-  | ExtBuiltin MultiplyInteger 
-      [ Constant (@Some _ DefaultUniInteger (ValueOf _ y)) 
-      ; Constant (@Some _ DefaultUniInteger (ValueOf _ x))
-      ] 
-      => Datatypes.Some (constInt (x * y))
+  | (Apply 
+      (Apply 
+        (Builtin MultiplyInteger) 
+        (Constant (@Some _ DefaultUniInteger (ValueOf _ x)))
+      ) 
+      (Constant (@Some _ DefaultUniInteger (ValueOf _ y)))
+    ) => Datatypes.Some (constInt (x * y))
   (* DivideInteger *)
-  | ExtBuiltin DivideInteger 
-      [ Constant (@Some _ DefaultUniInteger (ValueOf _ y)) 
-      ; Constant (@Some _ DefaultUniInteger (ValueOf _ x))
-      ] 
-      => Datatypes.Some (constInt (x / y))
+  | (Apply 
+      (Apply 
+        (Builtin DivideInteger) 
+        (Constant (@Some _ DefaultUniInteger (ValueOf _ x)))
+      ) 
+      (Constant (@Some _ DefaultUniInteger (ValueOf _ y)))
+    ) => Datatypes.Some (constInt (x / y))
   (* QuotientInteger *)
-  | ExtBuiltin QuotientInteger 
-      [ Constant (@Some _ DefaultUniInteger (ValueOf _ y))
-      ; Constant (@Some _ DefaultUniInteger (ValueOf _ x))
-      ] 
-      => Datatypes.Some (constInt (x ÷ y))
+  | (Apply 
+      (Apply 
+        (Builtin QuotientInteger) 
+        (Constant (@Some _ DefaultUniInteger (ValueOf _ x)))
+      ) 
+      (Constant (@Some _ DefaultUniInteger (ValueOf _ y)))
+    ) => Datatypes.Some (constInt (x ÷ y))
   (* RemainderInteger *)
-  | ExtBuiltin RemainderInteger 
-      [ Constant (@Some _ DefaultUniInteger (ValueOf _ y))
-      ; Constant (@Some _ DefaultUniInteger (ValueOf _ x))
-      ]
-      => Datatypes.Some (constInt (Z.rem x y))
+  | (Apply 
+      (Apply 
+        (Builtin RemainderInteger) 
+        (Constant (@Some _ DefaultUniInteger (ValueOf _ x)))
+      ) 
+      (Constant (@Some _ DefaultUniInteger (ValueOf _ y)))
+    ) => Datatypes.Some (constInt (Z.rem x y))
   (* ModInteger *)
-  | ExtBuiltin ModInteger 
-      [ Constant (@Some _ DefaultUniInteger (ValueOf _ y))
-      ; Constant (@Some _ DefaultUniInteger (ValueOf _ x))
-      ] 
-      => Datatypes.Some (constInt (x mod y))
+  | (Apply 
+      (Apply 
+        (Builtin ModInteger) 
+        (Constant (@Some _ DefaultUniInteger (ValueOf _ x)))
+      ) 
+      (Constant (@Some _ DefaultUniInteger (ValueOf _ y)))
+    ) => Datatypes.Some (constInt (x mod y))
   (** Binary predicates on integers *)
   (* LessThanInteger*)
-  | ExtBuiltin LessThanInteger 
-      [ Constant (@Some _ DefaultUniInteger (ValueOf _ y))
-      ; Constant (@Some _ DefaultUniInteger (ValueOf _ x))
-      ] 
-      => Datatypes.Some (constBool (x <? y))
+  | (Apply 
+      (Apply 
+        (Builtin LessThanInteger) 
+        (Constant (@Some _ DefaultUniInteger (ValueOf _ x)))
+      ) 
+      (Constant (@Some _ DefaultUniInteger (ValueOf _ y)))
+    ) => Datatypes.Some (constBool (x <? y))
   (* LessThanEqInteger *)
-  | ExtBuiltin LessThanEqInteger 
-      [ Constant (@Some _ DefaultUniInteger (ValueOf _ y)) 
-      ; Constant (@Some _ DefaultUniInteger (ValueOf _ x))
-      ] 
-      => Datatypes.Some (constBool (x <=? y))
+  | (Apply 
+      (Apply 
+        (Builtin LessThanEqInteger) 
+        (Constant (@Some _ DefaultUniInteger (ValueOf _ x)))
+      ) 
+      (Constant (@Some _ DefaultUniInteger (ValueOf _ y)))
+    ) => Datatypes.Some (constBool (x <=? y))
   (* GreaterThanInteger *)
-  | ExtBuiltin GreaterThanInteger 
-      [ Constant (@Some _ DefaultUniInteger (ValueOf _ y)) 
-      ; Constant (@Some _ DefaultUniInteger (ValueOf _ x))
-      ] 
-      => Datatypes.Some (constBool (x >? y))
+  | (Apply 
+      (Apply 
+        (Builtin GreaterThanInteger) 
+        (Constant (@Some _ DefaultUniInteger (ValueOf _ x)))
+      ) 
+      (Constant (@Some _ DefaultUniInteger (ValueOf _ y)))
+    ) => Datatypes.Some (constBool (x >? y))
   (* GreaterThanEqInteger *)
-  | ExtBuiltin GreaterThanEqInteger 
-      [ Constant (@Some _ DefaultUniInteger (ValueOf _ y)) 
-      ; Constant (@Some _ DefaultUniInteger (ValueOf _ x))
-      ] 
-      => Datatypes.Some (constBool (x >=? y))
+  | (Apply 
+      (Apply 
+        (Builtin GreaterThanEqInteger) 
+        (Constant (@Some _ DefaultUniInteger (ValueOf _ x)))
+      ) 
+      (Constant (@Some _ DefaultUniInteger (ValueOf _ y)))
+    ) => Datatypes.Some (constBool (x >=? y))
   (* EqInteger *)
-  | ExtBuiltin EqInteger 
-      [ Constant (@Some _ DefaultUniInteger (ValueOf _ y)) 
-      ; Constant (@Some _ DefaultUniInteger (ValueOf _ x))
-      ] 
-      => Datatypes.Some (constBool (x =? y))
+  | (Apply 
+      (Apply 
+        (Builtin EqInteger) 
+        (Constant (@Some _ DefaultUniInteger (ValueOf _ x)))
+      ) 
+      (Constant (@Some _ DefaultUniInteger (ValueOf _ y)))
+    ) => Datatypes.Some (constBool (x =? y))
   (** Bytestring operations *)
   (* Concatenate *)
-  | ExtBuiltin Concatenate
-      [ Constant (@Some _ DefaultUniByteString (ValueOf _ bs2))
-      ; Constant (@Some _ DefaultUniByteString (ValueOf _ bs1))
-      ]
-      => Datatypes.Some (constBS (bs1 ++ bs2))
+  | (Apply 
+      (Apply
+        (Builtin Concatenate)
+        (Constant (@Some _ DefaultUniByteString (ValueOf _ bs1)))    
+      )
+      (Constant (@Some _ DefaultUniByteString (ValueOf _ bs2)))
+    ) => Datatypes.Some (constBS (bs1 ++ bs2))
   (* TakeByteString *)
-  | ExtBuiltin TakeByteString
-      [ Constant (@Some _ DefaultUniByteString (ValueOf _ bs))
-      ; Constant (@Some _ DefaultUniInteger (ValueOf _ x))
-      ]
-      => Datatypes.Some (constBS (take x bs))
+  | (Apply 
+      (Apply
+        (Builtin TakeByteString)
+        (Constant (@Some _ DefaultUniInteger (ValueOf _ x)))    
+      )
+      (Constant (@Some _ DefaultUniByteString (ValueOf _ bs)))
+    ) => Datatypes.Some (constBS (take x bs))
   (* DropByteString *)
-  | ExtBuiltin DropByteString
-      [ Constant (@Some _ DefaultUniByteString (ValueOf _ bs))
-      ; Constant (@Some _ DefaultUniInteger (ValueOf _ x))
-      ]
-      => Datatypes.Some (constBS (drop x bs))
+  | (Apply 
+      (Apply
+        (Builtin DropByteString)
+        (Constant (@Some _ DefaultUniInteger (ValueOf _ x)))    
+      )
+      (Constant (@Some _ DefaultUniByteString (ValueOf _ bs)))
+    ) => Datatypes.Some (constBS (drop x bs))
   (** Bytestring hashing
       
       Note: We model hashing by identity. Comparing hashes now becomes a straightforward equality check.
       We believe modelling hash function as such is sufficient, because the dynamic semantics is not meant to 
       be used as a basis for a real-world evaluator.
   *)
-  | ExtBuiltin SHA2
-      [ Constant (@Some _ DefaultUniByteString (ValueOf _ bs))
-      ]
-      => Datatypes.Some (constBS bs)
-  | ExtBuiltin SHA3
-      [ Constant (@Some _ DefaultUniByteString (ValueOf _ bs))
-      ]
-      => Datatypes.Some (constBS bs)
+  | (Apply
+      (Builtin SHA2)
+      (Constant (@Some _ DefaultUniByteString (ValueOf _ bs)))
+    ) => Datatypes.Some (constBS bs)
+  | (Apply
+      (Builtin SHA3)
+      (Constant (@Some _ DefaultUniByteString (ValueOf _ bs)))
+    ) => Datatypes.Some (constBS bs)
   (** Signature verification 
       
       TODO: Obviously, this should evaluate to true. However, how can we model the verification of signatures? 
       Implementation of signature verification:
       https://input-output-hk.github.io/ouroboros-network/cardano-crypto/Crypto-ECC-Ed25519Donna.html
   *)
-  | ExtBuiltin VerifySignature
-      [ Constant (@Some _ DefaultUniByteString (ValueOf _ signature))
-      ; Constant (@Some _ DefaultUniByteString (ValueOf _ message))
-      ; Constant (@Some _ DefaultUniByteString (ValueOf _ publicKey))
-      ]
-      => Datatypes.Some (constBool true)
+  | (Apply 
+      (Apply
+        (Apply 
+          (Builtin VerifySignature)
+          (Constant (@Some _ DefaultUniByteString (ValueOf _ publicKey)))
+        )
+        (Constant (@Some _ DefaultUniByteString (ValueOf _ message)))
+      )
+      (Constant (@Some _ DefaultUniByteString (ValueOf _ signature)))
+    ) => Datatypes.Some (constBool true)
   (** Binary predicates on bytestrings *)
   (* EqByteString *)
-  | ExtBuiltin EqByteString
-      [ Constant (@Some _ DefaultUniByteString (ValueOf _ bs2))
-      ; Constant (@Some _ DefaultUniByteString (ValueOf _ bs1))
-      ]
-      => Datatypes.Some (constBool (bs1 =? bs2)%string)
+  | (Apply 
+      (Apply
+        (Builtin EqByteString)
+        (Constant (@Some _ DefaultUniByteString (ValueOf _ bs1)))    
+      )
+      (Constant (@Some _ DefaultUniByteString (ValueOf _ bs2)))
+    ) => Datatypes.Some (constBool (bs1 =? bs2)%string)
   (* LtByteString *)
-  | ExtBuiltin LtByteString
-      [ Constant (@Some _ DefaultUniByteString (ValueOf _ bs2))
-      ; Constant (@Some _ DefaultUniByteString (ValueOf _ bs1))
-      ]
-      => Datatypes.Some (constBool (to_Z bs1 <? to_Z bs2))
+  | (Apply 
+      (Apply
+        (Builtin LtByteString)
+        (Constant (@Some _ DefaultUniByteString (ValueOf _ bs1)))    
+      )
+      (Constant (@Some _ DefaultUniByteString (ValueOf _ bs2)))
+    ) => Datatypes.Some (constBool (to_Z bs1 <? to_Z bs2))
   (* GtByteString *)
-  | ExtBuiltin GtByteString
-      [ Constant (@Some _ DefaultUniByteString (ValueOf _ bs2))
-      ; Constant (@Some _ DefaultUniByteString (ValueOf _ bs1))
-      ]
-      => Datatypes.Some (constBool (to_Z bs1 >? to_Z bs2))
+  | (Apply 
+      (Apply
+        (Builtin GtByteString)
+        (Constant (@Some _ DefaultUniByteString (ValueOf _ bs1)))    
+      )
+      (Constant (@Some _ DefaultUniByteString (ValueOf _ bs2)))
+    ) => Datatypes.Some (constBool (to_Z bs1 >? to_Z bs2))
   (* String operations *)
   (* CharToString *)
-  | ExtBuiltin CharToString
-      [ Constant (@Some _ DefaultUniChar (ValueOf _ ch))
-      ]
-      => Datatypes.Some (constString (String ch EmptyString))
+  | (Apply
+      (Builtin CharToString)
+      (Constant (@Some _ DefaultUniChar (ValueOf _ ch)))  
+    ) => Datatypes.Some (constString (String ch EmptyString))
   (* Append *)
-  | ExtBuiltin Append
-      [ Constant (@Some _ DefaultUniString (ValueOf _ s2))
-      ; Constant (@Some _ DefaultUniString (ValueOf _ s1))
-      ]
-      => Datatypes.Some (constString (s1 ++ s2))
+  | (Apply
+      (Apply
+        (Builtin Append)
+        (Constant (@Some _ DefaultUniString (ValueOf _ s1)))
+      )
+      (Constant (@Some _ DefaultUniString (ValueOf _ s2)))
+    ) => Datatypes.Some (constString (s1 ++ s2))
   (* Trace *)
-  | ExtBuiltin Trace
-      [ Constant (@Some _ DefaultUniString (ValueOf _ s))
-      ] 
-      => Datatypes.Some (constUnit tt)
+  | (Apply
+      (Builtin Trace)
+      (Constant (@Some _ DefaultUniString (ValueOf _ s))) 
+    ) => Datatypes.Some (constUnit tt)
   (* Catch-all: The argument term is not a fully applied builtin *)
   | _ => None
   end.
