src/Language/PlutusIR/Semantics/Static.v
@@ -24,3 +24,9 @@ Create HintDb typing.
 #[export] Hint Constructors Ty.appears_free_in : typing.
 #[export] Hint Constructors Term.appears_free_in : typing.
 #[export] Hint Constructors Annotation.appears_free_in : typing.
+#[export] Hint Resolve 
+  normalise_to_normal
+  normalisation__deterministic
+  normalisation__stable 
+  has_type__normal
+  : typing.
