src/Language/PlutusIR/Semantics/TypeSafety/SubstitutionPreservesTyping/TypeSubstitution.v
@@ -1,5 +1,6 @@
 Require Import PlutusCert.Language.PlutusIR.
 Import NamedTerm.
+
 Require Import PlutusCert.Language.PlutusIR.Semantics.Static.
 
 
@@ -8,89 +9,48 @@ Theorem substituteT_preserves_kinding : forall T Delta X K U L,
   (X |-> L; Delta) |-* T : K ->
   empty |-* U : L ->
   Delta |-* (substituteT X U T) : K.
-Proof.
-  intros T Delta X K U L Hkind Hkind'.
-  generalize dependent L.
-  generalize dependent U.
-  generalize dependent K.
-  generalize dependent X.
-  generalize dependent Delta.
-
+Proof with eauto with typing.
   induction T.
+  all: intros Delta X K U L Hkind__T HHkind__U.
+  all: autorewrite with substituteTCA.
+  all: simpl.
+  all: inversion Hkind__T; subst...
   - (* Ty_Var *)
-    intros.
     rename t into Y.
-    inversion Hkind. subst.
-    simpl.
-    destruct (X =? Y) eqn:Heqb.
+    destruct (X =? Y)%string eqn:Heqb.
     + (* X = Y *)
       apply eqb_eq in Heqb as Heq.
       subst.
-      apply weakening_empty__has_kind.
+      apply Kinding.weakening_empty.
       rewrite update_eq in H1.
       inversion H1.
-      subst.
-      apply Hkind'.
+      subst...
     + (* X <> Y *)
       apply eqb_neq in Heqb as Hneq.
-      rewrite update_neq in H1; auto.
-      auto with typing.
-  - (* Ty_Fun *)
-    intros.
-    inversion Hkind. subst.
-    simpl.
-    eauto with typing.
-  - (* Ty_IFix *)
-    intros.
-    inversion Hkind. subst.
-    simpl.
-    eauto with typing.
+      rewrite update_neq in H1...
   - (* Ty_Forall *)
-    intros.
     rename b into bX.
-    inversion Hkind. subst.
-    simpl.
-    destruct (X =? bX) eqn:Heqb.
+    destruct (X =? bX)%string eqn:Heqb.
     + (* X = bX *)
       apply eqb_eq in Heqb as Heq.
       subst.
-      apply K_Forall.
-      rewrite update_shadow in H4.
-      assumption.
+      apply K_Forall...
+      rewrite update_shadow in H4...
     + (* X <> bX *)
       apply eqb_neq in Heqb as Hneq.
       apply K_Forall.
-      eapply IHT; eauto.
-      rewrite update_permute.
-      assumption.
-      auto.
-  - (* Ty_Builtin *)
-    intros.
-    inversion Hkind. subst.
-    simpl.
-    apply K_Builtin.
-    reflexivity.
+      eapply IHT...
+      rewrite update_permute...
   - (* Ty_Lam *)  
-    intros.
-    inversion Hkind. subst.
     rename b into bX.
-    simpl.
-    destruct (X =? bX) eqn:Heqb.
+    destruct (X =? bX)%string eqn:Heqb.
     + (* X = bX *)
       apply eqb_eq in Heqb as Heq.
       subst.
       apply K_Lam.
-      rewrite update_shadow in H4.
-      assumption.
+      rewrite update_shadow in H4...
     + (* X <> bX *)
       apply eqb_neq in Heqb as Hneq.
       apply K_Lam.
-      rewrite update_permute in H4.
-      eauto.
-      assumption.
-  - (* Ty_App *)
-    intros. 
-    inversion Hkind. subst.
-    simpl.
-    eauto with typing.
+      rewrite update_permute in H4...
 Qed.
